Port parsing and printing from rocq dir

hol/imp_printingScript.sml
@@ -3,7 +3,15 @@ Ancestors
   arithmetic list pair finite_map string words
   imp_source_syntax printing
 
-(* S-expression type for pretty printing IMP programs *)
+(* Pretty printer for imperative (IMP) programs.
+   Direct port of coq/theories/imperative/Printing.v.
+   Prints an IMP program as s-expression concrete syntax.
+   (ascii_name / name2str / num2str are reused from Theory printing.) *)
+
+
+(* ------------------------------------------------------------------ *)
+(* S-expression intermediate representation                            *)
+(* ------------------------------------------------------------------ *)
 
 Datatype:
   sexpr = SNum num
@@ -12,8 +20,6 @@ Datatype:
         | SPair sexpr sexpr
         | SEmpty
 End
-
-(* Helper constructors for common s-expression patterns *)
 
 Definition unary_sexpr_def:
   unary_sexpr op v = SBlock (SPair (SStr op) v)
@@ -37,7 +43,10 @@ Definition name_sexpr_def:
   name_sexpr n = SStr (name2str n)
 End
 
-(* Expression to s-expression *)
+
+(* ------------------------------------------------------------------ *)
+(* Expressions                                                         *)
+(* ------------------------------------------------------------------ *)
 
 Definition exp2s_def:
   exp2s (Var n)      = unary_sexpr "var" (name_sexpr n) ∧
@@ -57,7 +66,10 @@ Definition exps2s_def:
   exps2s es = SBlock (exps2s_imp es)
 End
 
-(* Comparison and test to s-expression *)
+
+(* ------------------------------------------------------------------ *)
+(* Comparisons and tests                                              *)
+(* ------------------------------------------------------------------ *)
 
 Definition cmp2str_def:
   cmp2str imp_source_syntax$Less  = "<" ∧
@@ -71,7 +83,10 @@ Definition test2s_def:
   test2s (Not t)        = unary_sexpr "not" (test2s t)
 End
 
-(* Parameter name list to s-expression *)
+
+(* ------------------------------------------------------------------ *)
+(* Parameter name lists                                               *)
+(* ------------------------------------------------------------------ *)
 
 Definition names2s_imp_def:
   names2s_imp []      = SEmpty ∧
@@ -82,27 +97,33 @@ Definition names2s_def:
   names2s ns = SBlock (names2s_imp ns)
 End
 
-(* Command to s-expression *)
+
+(* ------------------------------------------------------------------ *)
+(* Commands                                                           *)
+(* ------------------------------------------------------------------ *)
 
 Definition cmd2s_def:
-  cmd2s Skip              = SStr "skip" ∧
-  cmd2s (Seq c1 c2)       = SBlock (SPair (cmd2s c1) (cmd2s c2)) ∧
-  cmd2s (Assign n e)      = binary_sexpr "assign" (name_sexpr n) (exp2s e) ∧
-  cmd2s (Update a e e')   =
+  cmd2s Skip            = SStr "skip" ∧
+  cmd2s (Seq c1 c2)     = SBlock (SPair (cmd2s c1) (cmd2s c2)) ∧
+  cmd2s (Assign n e)    = binary_sexpr "assign" (name_sexpr n) (exp2s e) ∧
+  cmd2s (Update a e e') =
     ternary_sexpr "update" (exp2s a) (exp2s e) (exp2s e') ∧
-  cmd2s (If t c1 c2)      =
+  cmd2s (If t c1 c2)    =
     ternary_sexpr "if" (test2s t) (cmd2s c1) (cmd2s c2) ∧
-  cmd2s (While t c)       = binary_sexpr "while" (test2s t) (cmd2s c) ∧
-  cmd2s (Call n f es)     =
+  cmd2s (While t c)     = binary_sexpr "while" (test2s t) (cmd2s c) ∧
+  cmd2s (Call n f es)   =
     ternary_sexpr "call" (name_sexpr n) (name_sexpr f) (exps2s es) ∧
-  cmd2s (Return e)        = unary_sexpr "return" (exp2s e) ∧
-  cmd2s (Alloc n e)       = binary_sexpr "alloc" (name_sexpr n) (exp2s e) ∧
-  cmd2s (GetChar n)       = unary_sexpr "getchar" (name_sexpr n) ∧
-  cmd2s (PutChar e)       = unary_sexpr "putchar" (exp2s e) ∧
-  cmd2s Abort             = SBlock (SStr "abort")
+  cmd2s (Return e)      = unary_sexpr "return" (exp2s e) ∧
+  cmd2s (Alloc n e)     = binary_sexpr "alloc" (name_sexpr n) (exp2s e) ∧
+  cmd2s (GetChar n)     = unary_sexpr "getchar" (name_sexpr n) ∧
+  cmd2s (PutChar e)     = unary_sexpr "putchar" (exp2s e) ∧
+  cmd2s Abort           = SBlock (SStr "abort")
 End
 
-(* Function and program to s-expression *)
+
+(* ------------------------------------------------------------------ *)
+(* Functions and programs                                             *)
+(* ------------------------------------------------------------------ *)
 
 Definition func2s_def:
   func2s (Func n params body) =
@@ -110,27 +131,46 @@ Definition func2s_def:
       (SBlock (cmd2s body))
 End
 
-Definition funcs2s_def:
-  funcs2s []      = SEmpty ∧
-  funcs2s (f::fs) = SPair (func2s f) (funcs2s fs)
+Definition funcs2s_imp_def:
+  funcs2s_imp []      = SEmpty ∧
+  funcs2s_imp (f::fs) = SPair (func2s f) (funcs2s_imp fs)
 End
 
 Definition prog2s_def:
-  prog2s (Program funcs) = funcs2s funcs
+  prog2s (Program funcs) = funcs2s_imp funcs
 End
 
-(* Convert s-expression to string *)
+
+(* ------------------------------------------------------------------ *)
+(* Flattening an s-expression to a string via an append list          *)
+(* ------------------------------------------------------------------ *)
+
+Datatype:
+  str_app_list = StrList (char list)
+               | StrAppend str_app_list str_app_list
+End
 
 Definition sexpr2str_def:
-  sexpr2str (SNum n)      = "'" ++ num2str n ∧
-  sexpr2str (SStr s)      = s ∧
-  sexpr2str (SPair s1 s2) = sexpr2str s1 ++ " " ++ sexpr2str s2 ∧
-  sexpr2str SEmpty        = "" ∧
-  sexpr2str (SBlock s)    = "(" ++ sexpr2str s ++ ")"
+  sexpr2str (SNum n)      = StrAppend (StrList "'") (StrList (num2str n)) ∧
+  sexpr2str (SStr s)      = StrList s ∧
+  sexpr2str (SPair s1 s2) =
+    StrAppend (sexpr2str s1) (StrAppend (StrList " ") (sexpr2str s2)) ∧
+  sexpr2str SEmpty        = StrList "" ∧
+  sexpr2str (SBlock s)    =
+    StrAppend (StrList "(") (StrAppend (sexpr2str s) (StrList ")"))
 End
 
-(* Top-level: IMP program to string *)
+Definition flatten_str_app_list_def:
+  flatten_str_app_list (StrList s)       = s ∧
+  flatten_str_app_list (StrAppend s1 s2) =
+    flatten_str_app_list s1 ++ flatten_str_app_list s2
+End
+
+
+(* ------------------------------------------------------------------ *)
+(* Top-level: IMP program to string                                   *)
+(* ------------------------------------------------------------------ *)
 
 Definition imp2str_def:
-  imp2str p = sexpr2str (prog2s p)
+  imp2str p = flatten_str_app_list (sexpr2str (prog2s p))
 End
