hol/imp_parsingScript.sml
@@ -2,278 +2,249 @@ Theory imp_parsing
 Ancestors
   arithmetic list pair finite_map string words
   source_values imp_source_syntax
+Libs
+  BasicProvers
 
+(* Lexer and parser for imperative (IMP) programs.
+   Direct port of coq/theories/parsing/Parser.v (+ ParserData.v).
+   The concrete syntax is s-expressions; values (source_values$v) are
+   used as the intermediate tree, exactly as in the Rocq development. *)
+
+
+(* ------------------------------------------------------------------ *)
+(* Tokens (coq: parsing/ParserData.v)                                 *)
+(* ------------------------------------------------------------------ *)
 
 Datatype:
-  keyword = If | While | Else | Return | Abort | Add | Sub | Div |
-            Less | Equal | Or | And | Not | Alloc | GetChar | PutChar
+  token = OPEN | CLOSE | DOT | NUM num | QUOTE num
 End
 
-Datatype:
-  token = Ident num
-        | Lit num
-        | ParenOpen
-        | ParenClose
-        | BraceOpen
-        | BraceClose
-        | BracketOpen
-        | BracketClose
-        | Keyword keyword
-        | Semicolon
-        | Comma
+
+(* ------------------------------------------------------------------ *)
+(* Lexing (coq: read_nmc / read_alp / end_line / lex / lexer)         *)
+(* read_num generalises read_nmc ("0".."9", base 10) and              *)
+(* read_alp ("*".."z", base 256) into a single reader.                *)
+(* ------------------------------------------------------------------ *)
+
+Definition read_num_def:
+  read_num l h f x acc [] = (acc,[]) ∧
+  read_num l h f x acc (c::cs) =
+    if ORD l ≤ ORD c ∧ ORD c ≤ ORD h then
+      read_num l h f x (f * acc + (ORD c - x)) cs
+    else (acc,c::cs)
 End
 
-Definition add_parens_def:
-  add_parens xs = if LENGTH xs = 1 then xs else [ParenOpen] ++ xs ++ [ParenClose]
-End
-
-Definition e2t_def:
-  e2t (Var n)      = [Ident n] ∧
-  e2t (Const c)    = [Lit (w2n c)] ∧
-  e2t (Add e1 e2)  = add_parens (e2t e1) ++ [Keyword Add] ++ add_parens (e2t e2) ∧
-  e2t (Sub e1 e2)  = add_parens (e2t e1) ++ [Keyword Sub] ++ add_parens (e2t e2) ∧
-  e2t (Div e1 e2)  = add_parens (e2t e1) ++ [Keyword Div] ++ add_parens (e2t e2) ∧
-  e2t (Read e1 e2) = add_parens (e2t e1) ++ [BracketOpen] ++ e2t e2 ++ [BracketClose]
-End
-
-Definition find_end_def:
-  find_end [] d acc = (REVERSE acc,[]) ∧
-  find_end (x::xs) d acc =
-    case x of
-    | ParenClose => if d = 0 then (REVERSE acc, xs) else find_end xs (d-1) (x::acc)
-    | ParenOpen => find_end xs (d+1) (x::acc)
-    | _ => find_end xs d (x::acc)
-End
-
-Theorem find_end_length:
-  ∀xs k acc ys zs.
-    find_end xs k acc = (ys,zs) ⇒
-    LENGTH ys + LENGTH zs ≤ LENGTH xs + LENGTH acc
+Theorem read_num_length:
+  ∀l h xs n ys f acc x.
+    read_num l h f x acc xs = (n,ys) ⇒
+    LENGTH ys ≤ LENGTH xs ∧ (xs ≠ ys ⇒ LENGTH ys < LENGTH xs)
 Proof
-  Induct \\ fs [find_end_def,AllCaseEqs()] \\ rw [] \\ res_tac \\ fs []
+  Induct_on ‘xs’ \\ rw [read_num_def]
+  \\ TRY pairarg_tac \\ fs [] \\ rw [] \\ res_tac \\ fs []
 QED
 
-Definition read_fst_def:
-  read_fst xs =
-    case xs of
-    | (ParenOpen :: ys) => find_end ys 0 []
-    | (Ident n :: ys) => ([Ident n],ys)
-    | (Lit w :: ys) => ([Lit w],ys)
-    | _ => ([],[])
+Definition end_line_def:
+  end_line [] = [] ∧
+  end_line (c::cs) = if c = #"\n" then cs else end_line cs
 End
 
-Definition k2e_def:
-  k2e Add e1 e2 = Add e1 e2 ∧
-  k2e Sub e1 e2 = Sub e1 e2 ∧
-  k2e Div e1 e2 = Div e1 e2 ∧
-  k2e (k:keyword) e1 e2 = Add e1 e2
-End
-
-Definition front_def:
-  front [] = [] ∧
-  front (x::xs) = if NULL xs then [] else x :: front xs
-End
-
-Theorem LENGTH_front:
-  ∀xs. LENGTH (front xs) = LENGTH xs - 1
+Theorem end_line_length:
+  ∀cs. STRLEN (end_line cs) < SUC (STRLEN cs)
 Proof
-  Induct \\ fs [front_def] \\ rw [] \\ Cases_on ‘xs’ \\ fs []
+  Induct \\ rw [end_line_def]
 QED
 
-Theorem front_snoc:
-  ∀xs x. front (xs ++ [x]) = xs
-Proof
-  Induct \\ fs [front_def]
-QED
-
-Definition t2e_def:
-  t2e xs =
-    if LENGTH xs < 2 then
-      (case xs of
-       | (Ident n :: _) => Var n
-       | (Lit n :: _) => Const (n2w n)
-       | _ => Const 0w)
-    else
-      let (ys,zs) = read_fst xs in
-      let e1 = t2e ys in
-        case zs of
-        | (BracketOpen::ts) => Read e1 (t2e (front ts))
-        | (Keyword k::ts) => k2e k e1 (t2e ts)
-        | _ => e1
+Definition lex_def:
+  lex q [] acc = acc ∧
+  lex q (c::cs) acc =
+      if MEM c " \t\n" then lex NUM cs acc else
+      if c = #"#" then lex NUM (end_line cs) acc else
+      if c = #"." then lex NUM cs (DOT::acc) else
+      if c = #"(" then lex NUM cs (OPEN::acc) else
+      if c = #")" then lex NUM cs (CLOSE::acc) else
+      if c = #"'" then lex QUOTE cs acc else
+        let (n,rest) = read_num #"0" #"9" 10 (ORD #"0") 0 (c::cs) in
+          if rest ≠ c::cs then lex NUM rest (q n::acc) else
+            let (n,rest) = read_num #"*" #"z" 256 0 0 (c::cs) in
+              if rest ≠ c::cs then lex NUM rest (q n::acc) else
+                lex NUM cs acc
 Termination
-  WF_REL_TAC ‘measure LENGTH’ \\ rw []
-  \\ gvs [read_fst_def,AllCaseEqs()]
-  \\ imp_res_tac find_end_length \\ fs [LENGTH_front]
+  WF_REL_TAC ‘measure (LENGTH o FST o SND)’ \\ rw []
+  \\ imp_res_tac (GSYM read_num_length) \\ fs [end_line_length]
 End
 
-Inductive balanced:
-[~nil:]
-  balanced []
-[~single:]
-  (∀x. x ≠ ParenOpen ∧ x ≠ ParenClose ⇒ balanced [x])
-[~append:]
-  (∀xs ys. balanced xs ∧ balanced ys ⇒ balanced (xs ++ ys))
-[~paren:]
-  (∀xs. balanced xs ⇒ balanced ([ParenOpen] ++ xs ++ [ParenClose]))
+Definition lexer_def:
+  lexer input = lex NUM input []
 End
 
-(* Theorem find_end_lemma:
-  ∀xs ys d acc.
-    balanced xs ⇒
-    find_end (xs ++ ys) d acc = find_end ys d (REVERSE xs ++ acc)
-Proof
-  Induct_on ‘balanced’ \\ rw []
-  >- (Cases_on ‘x’ \\ fs [find_end_def])
-  >- asm_rewrite_tac [GSYM APPEND_ASSOC,REVERSE_APPEND]
-  \\ simp [find_end_def] \\ asm_rewrite_tac [GSYM APPEND_ASSOC,REVERSE_APPEND,APPEND]
-  \\ simp [find_end_def] \\ asm_rewrite_tac [GSYM APPEND_ASSOC,APPEND]
-QED
 
-Theorem balanced_add_parens:
-  balanced xs ⇒ balanced (add_parens xs)
-Proof
-  rw [add_parens_def] \\ simp [Once balanced_cases]
-QED
+(* ------------------------------------------------------------------ *)
+(* Parsing tokens into a value tree (coq: quote / parse)              *)
+(* ------------------------------------------------------------------ *)
 
-Theorem balanced_e2t:
-  ∀e. balanced (e2t e)
-Proof
-  Induct \\ fs [e2t_def]
-  >- simp [Once balanced_cases]
-  >- simp [Once balanced_cases]
-  \\ rpt $ irule_at Any balanced_append
-  \\ rpt $ irule_at Any balanced_add_parens
-  \\ simp [] \\ rpt $ simp [Once balanced_cases]
-QED
-
-Theorem read_fst_lemma:
-  ∀e ys. read_fst (add_parens (e2t e) ++ ys) = (e2t e,ys)
-Proof
-  fs [read_fst_def] \\ rw [add_parens_def]
-  >- (pop_assum mp_tac \\ Cases_on ‘e’ \\ fs [e2t_def]
-      \\ simp [Once t2e_def] \\ rw [add_parens_def])
-  \\ rewrite_tac [GSYM APPEND_ASSOC,APPEND]
-  \\ qspec_then ‘e’ assume_tac balanced_e2t
-  \\ drule find_end_lemma \\ fs [find_end_def]
-QED
-
-Theorem t2e_add_parens:
-  t2e (add_parens (e2t e)) = t2e (e2t e)
-Proof
-  simp [Once t2e_def]
-  \\ qspecl_then [‘e’,‘[]’] mp_tac read_fst_lemma \\ fs []
-  \\ rw [] \\ fs [add_parens_def] \\ rw [] \\ fs []
-  \\ pop_assum mp_tac \\ Cases_on ‘e’ \\ fs [e2t_def] \\ simp [Once t2e_def]
-QED
-
-Theorem t2e_e2t:
-  ∀e. t2e (e2t e) = e
-Proof
-  Induct \\ simp [Once t2e_def,e2t_def]
-  \\ ‘1 ≤ LENGTH (add_parens (e2t e))’ by rw [add_parens_def]
-  \\ rewrite_tac [GSYM APPEND_ASSOC,APPEND]
-  \\ simp [read_fst_lemma,k2e_def,front_snoc,t2e_add_parens]
-QED
-
-Definition test2t_def:
-  test2t _ = ARB
+Definition quote_def:
+  quote n = list [Num (name "'"); Num n]
 End
 
-Definition es2t_def:
-  es2t sep [] = [ParenClose] ∧
-  es2t sep (x::xs) = [sep] ++ e2t x ++ es2t Comma xs
+Definition parse_def:
+  parse [] x s = x ∧
+  parse (CLOSE :: rest) x s = parse rest (Num 0) (x::s) ∧
+  parse (OPEN :: rest) x s =
+    (case s of [] => parse rest x s
+     | (y::ys) => parse rest (Pair x y) ys) ∧
+  parse (NUM n :: rest) x s = parse rest (Pair (Num n) x) s ∧
+  parse (QUOTE n :: rest) x s = parse rest (Pair (quote n) x) s ∧
+  parse (DOT :: rest) x s = parse rest (head x) s
 End
 
-Definition args2t_def:
-  args2t xs = if NULL xs then [ParenOpen; ParenClose] else es2t ParenOpen xs
-End
 
-Definition c2t_def:
-  c2t []            = [BraceClose] ∧
-  c2t (x::y::ys)    = c2t [x] ++ c2t (y::ys) ∧
-  c2t [Assign n e]  = [Ident n; Keyword Equal] ++ e2t e ++ [Semicolon] ∧
-  c2t [Return e]    = [Keyword Return] ++ e2t e ++ [Semicolon] ∧
-  c2t [Abort]       = [Keyword Abort; Semicolon] ∧
-  c2t [PutChar e]   = [Keyword PutChar; ParenOpen] ++ e2t e ++ [ParenClose; Semicolon] ∧
-  c2t [GetChar n]   = [Ident n; Keyword Equal; Keyword GetChar;
-                       ParenOpen; ParenClose; Semicolon] ∧
-  c2t [If t c1 c2]  = [Keyword If; ParenOpen] ++ test2t t ++ [ParenClose; BraceOpen] ++
-                       c2t c1 ++ [Keyword Else; BraceOpen] ++ c2t c2 ∧
-  c2t [While t c]   = [Keyword While; ParenOpen] ++ test2t t ++ [ParenClose; BraceOpen] ++
-                       c2t c ∧
-  (*    | Update exp exp exp              a[e] := e'              *)
-  c2t [Call v n es] = [Ident v; Keyword Equal; Ident n] ++ args2t es ++ [Semicolon] ∧
-  c2t [Alloc v e]   = [Ident v; Keyword Equal; Keyword Alloc] ++ e2t e ++ [Semicolon]
+(* ------------------------------------------------------------------ *)
+(* Converting a value tree into IMP abstract syntax                    *)
+(* (coq: v2list / num2exp / v2exp / vs2exps / v2cmp / v2test /         *)
+(*        v2cmd / vs2args / v2func / v2funcs / vs2prog)                *)
+(* ------------------------------------------------------------------ *)
+
+Definition v2list_def:
+  v2list v = if isNum v then [] else head v :: v2list (tail v)
 Termination
-  WF_REL_TAC ‘measure $ list_size cmd_size’
-End *)
+  WF_REL_TAC ‘measure v_size’ \\ Cases \\ fs []
+End
 
-(*
+Definition num2exp_def:
+  num2exp n =
+    if is_upper n then
+      (if 18446744073709551615 < n then Const 0w else Const (n2w n))
+    else Var n
+End
 
-Definition rhs2c_def:
-  rhs2c n xs =
-    case xs of
-    | [] => ([],xs)
-    | (Keyword k :: ys) =>
-         (case k of
-          | Alloc => )
+Definition v2exp_def:
+  v2exp v =
+    case v of
+    | Num n => num2exp n
+    | Pair v0 (Num _) => num2exp (getNum v0)
+    | Pair v0 (Pair v1 v2) =>
+        let n = getNum v0 in
+          if n = name "'" then
+            (if 18446744073709551615 < getNum v1 then Const 0w
+             else Const (n2w (getNum v1)))
+          else if n = name "var" then Var (getNum v1)
+          else case v2 of
+               | Num _ => num2exp n
+               | Pair v2 v3 =>
+                   if n = name "+" then Add (v2exp v1) (v2exp v2)
+                   else if n = name "-" then Sub (v2exp v1) (v2exp v2)
+                   else if n = name "div" then Div (v2exp v1) (v2exp v2)
+                   else if n = name "read" then Read (v2exp v1) (v2exp v2)
+                   else num2exp n
+Termination
+  WF_REL_TAC ‘measure v_size’ \\ simp [v_size_def]
+End
 
-    |
+Definition vs2exps_def:
+  vs2exps [] = [] ∧
+  vs2exps (v::vs) = v2exp v :: vs2exps vs
+End
 
-Definition t2c_def:
-  t2c (BraceClose::xs) acc = (REVERE acc,xs) ∧
-  t2c (Keyword k::xs) acc =
-    (case k of
-     | If => ARB
-     | While => ARB
-     | Return => ARB
-     | PutChar => ARB
-     | (* Abort *) _ => (REVERSE (Abort::acc),xs)) ∧
-  t2c (Ident n::xs) acc =
-    (let (cs.ys) = rhs2c n (TL xs) acc in
-       t2c ys (cs ++ acc))
-  t2c _ acc = (REVERSE acc,[])
+Definition v2cmp_def:
+  v2cmp v =
+    let n = getNum v in
+      if n = name "<" then imp_source_syntax$Less
+      else if n = name "=" then Equal
+      else imp_source_syntax$Less
+End
+
+Definition v2test_def:
+  v2test v =
+    case v of
+    | Num _ => Test imp_source_syntax$Less (Const 0w) (Const 0w)
+    | Pair v0 (Num _) => Test imp_source_syntax$Less (Const 0w) (Const 0w)
+    | Pair v0 (Pair v1 v2) =>
+        let n = getNum v0 in
+          if n = name "not" then Not (v2test v1)
+          else case v2 of
+               | Num _ => Test imp_source_syntax$Less (Const 0w) (Const 0w)
+               | Pair v2 v3 =>
+                   if n = name "and" then And (v2test v1) (v2test v2)
+                   else if n = name "or" then Or (v2test v1) (v2test v2)
+                   else Test (v2cmp v0) (v2exp v1) (v2exp v2)
+Termination
+  WF_REL_TAC ‘measure v_size’ \\ simp [v_size_def]
+End
+
+Definition v2cmd_def:
+  v2cmd v =
+    case v of
+    | Num _ => Skip
+    | Pair v0 v1 =>
+        if ~isNum v0 then
+          (if isNum v1 then v2cmd v0
+           else Seq (v2cmd v0) (v2cmd v1))
+        else
+          let n = getNum v0 in
+          if n = name "abort" then Abort
+          else case v1 of
+          | Num _ => Skip
+          | Pair v1 v2 =>
+              if n = name "return" then Return (v2exp v1)
+              else if n = name "getchar" then GetChar (getNum v1)
+              else if n = name "putchar" then PutChar (v2exp v1)
+              else case v2 of
+              | Num _ => Skip
+              | Pair v2 v3 =>
+                  if n = name "assign" then
+                    Assign (getNum v1) (v2exp v2)
+                  else if n = name "while" then
+                    While (v2test v1) (v2cmd v2)
+                  else if n = name "alloc" then
+                    Alloc (getNum v1) (v2exp v2)
+                  else case v3 of
+                  | Num _ =>
+                      Call (getNum v0) (getNum v1) (vs2exps (v2list v2))
+                  | Pair v3 v4 =>
+                      if n = name "update" then
+                        Update (v2exp v1) (v2exp v2) (v2exp v3)
+                      else if n = name "if" then
+                        If (v2test v1) (v2cmd v2) (v2cmd v3)
+                      else if n = name "call" then
+                        Call (getNum v1) (getNum v2) (vs2exps (v2list v3))
+                      else
+                        Call (getNum v0) (getNum v1)
+                             (vs2exps (v2list (Pair v2 v3)))
+Termination
+  WF_REL_TAC ‘measure v_size’ \\ simp [v_size_def]
+End
+
+Definition vs2args_def:
+  vs2args [] = [] ∧
+  vs2args (v::vs) = getNum v :: vs2args vs
+End
+
+Definition v2func_def:
+  v2func v =
+    let fname = getNum (el1 v) in
+    let args  = vs2args (v2list (el2 v)) in
+    let body  = v2cmd (el3 v) in
+      Func fname args body
+End
+
+Definition v2funcs_def:
+  v2funcs []      = [] ∧
+  v2funcs (v::vs) = v2func v :: v2funcs vs
+End
+
+Definition vs2prog_def:
+  vs2prog vs = Program (v2funcs vs)
 End
 
 
+(* ------------------------------------------------------------------ *)
+(* Entire parser (coq: parser / str2imp)                              *)
+(* ------------------------------------------------------------------ *)
 
-
-
-Datatype:
-  cmp = Less | Equal
+Definition parser_def:
+  parser tokens = vs2prog (v2list (parse tokens (Num 0) []))
 End
-
-Datatype:
-  test = Test cmp exp exp | And test test | Or test test | Not test
-End
-
-Datatype:
-  cmd = Assign name exp                (*  v := e                  *)
-      | Update exp exp exp             (*  a[e] := e'              *)
-      | If test (cmd list) (cmd list)  (*  if (test) ... else ...  *)
-      | While test (cmd list)          (*  while (test) ...        *)
-      | Call name name (exp list)      (*  v := foo(e1,e2,e3,...)  *)
-      | Return exp                     (*  return from function    *)
-      | Alloc name exp                 (*  v := malloc(e)          *)
-      | GetChar name                   (*  v := getchar()          *)
-      | PutChar exp                    (*  putchar(e)              *)
-      | Abort                          (*  exit(1)                 *)
-End
-
-Datatype:
-  func = Func name (name list) (cmd list)   (* func name, formal params, body *)
-End
-
-Datatype:
-  prog = Program (func list)    (*   a complete program is a list   *)
-End                             (*   of function definitions        *)
-
-Definition get_name_def[simp]:
-  get_name (Func n _ _) = n
-End
-
-*)
 
 Definition str2imp_def:
-  str2imp (s:string) = ARB : prog
+  str2imp str = parser (lexer str)
 End
