hol/imp_compiler_proofsScript.sml
@@ -3,7 +3,7 @@ Ancestors
   arithmetic list pair finite_map string words
   imp_source_syntax imp_source_semantics
   x64asm_syntax x64asm_semantics
-  imp_printing imp_sexp_parser imp_compiler
+  imp_printing imp_parsing imp_compiler
   imp_to_asm_proof source_to_imp
 Libs
   wordsLib BasicProvers
